theories/lang/cpp/bi/split_cv.v
@@ -16,7 +16,7 @@ Import ChargeNotation.
 (**
 Overview:
 
-- [SplitCV], [CombineCV] split and combine terms of type [CV.t] built
+- [SplitcQp], [CombinecQp] split and combine terms of type [cQp.t] built
 up from booleans, fractions, and [op]
 *)
 
@@ -29,20 +29,20 @@ should be opaque for typeclass resolution.
 #[local] Notation Cut := TCNoBackTrack.
 
 (**
-[SplitCV cv cv1 cv2] splits [cv : CV.t] into [cv1], [cv2] s.t. [cv =
+[SplitcQp cv cv1 cv2] splits [cv : cQp.t] into [cv1], [cv2] s.t. [cv =
 cv1 ⋅ cv2], adjusting the outputs [cv1], [cv2] for readabilty.
 *)
-Class SplitCV (cv cv1 cv2 : CV.t) : Prop := split_cv : cv = cv1 ⋅ cv2.
-#[global] Hint Mode SplitCV + - - : typeclass_instances.
-#[global] Arguments SplitCV : simpl never.
+Class SplitcQp (cv cv1 cv2 : cQp.t) : Prop := split_cv : cv = cv1 ⋅ cv2.
+#[global] Hint Mode SplitcQp + - - : typeclass_instances.
+#[global] Arguments SplitcQp : simpl never.
 #[global] Arguments split_cv _ {_ _ _} : assert.
 
 Module split_cv.
 
   (**
-  We use this auxiliary judgment to [Cut] in [SplitCV].
+  We use this auxiliary judgment to [Cut] in [SplitcQp].
   *)
-  Class Split (cv cv1 cv2 : CV.t) : Prop := split : cv = cv1 ⋅ cv2.
+  Class Split (cv cv1 cv2 : cQp.t) : Prop := split : cv = cv1 ⋅ cv2.
   #[global] Hint Mode Split + - - : typeclass_instances.
   #[global] Arguments Split : simpl never.
   #[global] Arguments split _ {_ _ _} : assert.
@@ -54,32 +54,32 @@ Module split_cv.
   #[global] Instance split_mk c c1 c2 q q1 q2 :
     SplitAndB c c1 c2 ->
     SplitFrac q q1 q2 ->
-    Split (CV.mk c q) (CV.mk c1 q1) (CV.mk c2 q2) | 10.
+    Split (cQp.mk c q) (cQp.mk c1 q1) (cQp.mk c2 q2) | 10.
   Proof.
-    intros. rewrite /Split CV.t_op/=. by f_equal.
+    intros. rewrite /Split cQp.t_op/=. by f_equal.
   Qed.
 
   #[global] Instance split_var cv c1 c2 cv1 cv2 :
-    SplitAndB (CV.is_const cv) c1 c2 ->
-    SplitFrac (CV.frac cv) cv1 cv2 ->
-    Split cv (CV.mk c1 cv1) (CV.mk c2 cv2) | 50.
+    SplitAndB (cQp.is_const cv) c1 c2 ->
+    SplitFrac (cQp.frac cv) cv1 cv2 ->
+    Split cv (cQp.mk c1 cv1) (cQp.mk c2 cv2) | 50.
   Proof.
-    intros. rewrite /Split CV.t_op/=. rewrite (CV.eta cv). by f_equal.
+    intros. rewrite /Split cQp.t_op/=. rewrite (cQp.eta cv). by f_equal.
   Qed.
 
 End split_cv.
 
 #[global] Instance split_cv_split cv cv1 cv2 :
-  split_cv.SPLIT cv cv1 cv2 -> SplitCV cv cv1 cv2 | 10.
+  split_cv.SPLIT cv cv1 cv2 -> SplitcQp cv cv1 cv2 | 10.
 Proof. by case. Qed.
 
 (**
-[CombineCV cv1 cv2 cv] combine [cv1, cv2 : CV.t] into [cv = cv1 ⋅ cv2],
+[CombinecQp cv1 cv2 cv] combine [cv1, cv2 : cQp.t] into [cv = cv1 ⋅ cv2],
 adjusting the output [cv] for readability.
 *)
-Class CombineCV (cv1 cv2 cv : CV.t) : Prop := combine_cv : cv1 ⋅ cv2 = cv.
-#[global] Hint Mode CombineCV + + - : typeclass_instances.
-#[global] Arguments CombineCV : simpl never.
+Class CombinecQp (cv1 cv2 cv : cQp.t) : Prop := combine_cv : cv1 ⋅ cv2 = cv.
+#[global] Hint Mode CombinecQp + + - : typeclass_instances.
+#[global] Arguments CombinecQp : simpl never.
 #[global] Arguments combine_cv _ _ {_ _} : assert.
 
 Module combine_cv.
@@ -87,30 +87,30 @@ Module combine_cv.
   (**
   Step 1: Combine the component parts, producing a possibly ugly term.
   *)
-  Class Combine (cv1 cv2 cv : CV.t) : Prop := combine : cv1 ⋅ cv2 = cv.
+  Class Combine (cv1 cv2 cv : cQp.t) : Prop := combine : cv1 ⋅ cv2 = cv.
   #[global] Hint Mode Combine + + - : typeclass_instances.
   #[global] Arguments Combine : simpl never.
   #[global] Arguments combine _ _ {_ _} : assert.
 
   #[global] Instance combine_mk_mk c1 c2 c q1 q2 q :
     CombineAndB c1 c2 c -> CombineFrac q1 q2 q ->
-    Combine (CV.mk c1 q1) (CV.mk c2 q2) (CV.mk c q) | 10.
+    Combine (cQp.mk c1 q1) (cQp.mk c2 q2) (cQp.mk c q) | 10.
   Proof.
-    intros. rewrite /Combine CV.t_op /=.
+    intros. rewrite /Combine cQp.t_op /=.
     by rewrite combine_andb combine_frac.
   Qed.
 
   #[global] Instance combine_mk_any c1 c cv1 cv2 :
-    CombineAndB c1 (CV.is_const cv2) c ->
-    Combine (CV.mk c1 cv1) cv2 (CV.mk c (cv1 + CV.frac cv2)) | 15.
+    CombineAndB c1 (cQp.is_const cv2) c ->
+    Combine (cQp.mk c1 cv1) cv2 (cQp.mk c (cv1 + cQp.frac cv2)) | 15.
   Proof.
-    intros. rewrite /Combine CV.t_op /=. by rewrite combine_andb.
+    intros. rewrite /Combine cQp.t_op /=. by rewrite combine_andb.
   Qed.
   #[global] Instance combine_any_mk c2 c cv2 cv1 :
-    CombineAndB (CV.is_const cv1) c2 c ->
-    Combine cv1 (CV.mk c2 cv2) (CV.mk c (CV.frac cv1 + cv2)) | 15.
+    CombineAndB (cQp.is_const cv1) c2 c ->
+    Combine cv1 (cQp.mk c2 cv2) (cQp.mk c (cQp.frac cv1 + cv2)) | 15.
   Proof.
-    intros. rewrite /Combine CV.t_op /=. by rewrite combine_andb.
+    intros. rewrite /Combine cQp.t_op /=. by rewrite combine_andb.
   Qed.
 
   #[global] Instance combine_any_any cv1 cv2 : Combine cv1 cv2 (cv1 ⋅ cv2) | 50.
@@ -120,12 +120,12 @@ Module combine_cv.
   Step 2: Make the term from step (1) prettier.
   *)
 
-  Class Prettify (cv' cv : CV.t) : Prop := prettify : cv' = cv.
+  Class Prettify (cv' cv : cQp.t) : Prop := prettify : cv' = cv.
   #[global] Hint Mode Prettify + - : typeclass_instances.
   #[global] Arguments Prettify : simpl never.
   #[global] Arguments prettify _ {_ _} : assert.
 
-  #[global] Instance prettify_eta c : Prettify (CV.mk (CV.is_const c) (CV.frac c)) c | 10.
+  #[global] Instance prettify_eta c : Prettify (cQp.mk (cQp.is_const c) (cQp.frac c)) c | 10.
   Proof. done. Qed.
   #[global] Instance prettify_skip c : Prettify c c | 50.
   Proof. done. Qed.
@@ -134,7 +134,7 @@ End combine_cv.
 
 #[global] Instance combine_cv_instance c1 c2 chat c :
   combine_cv.Combine c1 c2 chat -> combine_cv.Prettify chat c ->
-  CombineCV c1 c2 c | 10.
+  CombinecQp c1 c2 c | 10.
 Proof.
   by rewrite /combine_cv.Combine /combine_cv.Prettify=><-.
 Qed.
