theories/lang/cpp/bi/cfractional_tests.v
@@ -14,7 +14,7 @@ Import ChargeNotation.
 
 Section EXAMPLES.
   Context {PROP : bi}.
-  Context (R : CV.t -> PROP) `{!cfractional.CFractional R}.
+  Context (R : cQp.t -> PROP) `{!cfractional.CFractional R}.
 
   Let R_as_fractional q : AsCFractional (R q) R q.
   Proof. exact: Build_AsCFractional. Qed.
@@ -28,36 +28,36 @@ Section EXAMPLES.
     R (cv1 ⋅ cv2) |-- R cv1 ** R cv2.
   Proof. iIntros "[R1 R2]". by iFrame "R1 R2". Abort.
   Let split_cv_mk cv c q :
-    R (cv ⋅ CV.mk c q) |-- R cv ** R (CV.mk c q).
+    R (cv ⋅ cQp.mk c q) |-- R cv ** R (cQp.mk c q).
   Proof. iIntros "[R1 R2]". by iFrame "R1 R2". Abort.
   Let split_mk_cv cv c q :
-    R (CV.mk c q ⋅ cv) |-- R (CV.mk c q) ** R cv.
+    R (cQp.mk c q ⋅ cv) |-- R (cQp.mk c q) ** R cv.
   Proof. iIntros "[R1 R2]". by iFrame "R1 R2". Abort.
   Let split_mk_mk c1 c2 q1 q2 :
-    R (CV.mk c1 q1 ⋅ CV.mk c2 q2) |-- R (CV.mk c1 q1) ** R (CV.mk c2 q2).
+    R (cQp.mk c1 q1 ⋅ cQp.mk c2 q2) |-- R (cQp.mk c1 q1) ** R (cQp.mk c2 q2).
   Proof. iIntros "[R1 R2]". by iFrame "R1 R2". Abort.
 
   (**
-  Splitting [CV.is_const] knows about [&&].
+  Splitting [cQp.is_const] knows about [&&].
   *)
 
   Let split_andb c1 c2 q :
-    R (CV.mk (c1 && c2) q) |-- R (CV.mk c1 (q/2)) ** R (CV.mk c2 (q/2)).
+    R (cQp.mk (c1 && c2) q) |-- R (cQp.mk c1 (q/2)) ** R (cQp.mk c2 (q/2)).
   Proof. iIntros "[R1 R2]". by iFrame "R1 R2". Abort.
 
-  (** Otherwise, both sides get the same [CV.is_const] after the split. *)
+  (** Otherwise, both sides get the same [cQp.is_const] after the split. *)
 
   Let split_mut :
-    R (CV.mut 1) |-- R (CV.mut (1/2)) ** R (CV.mut (1/2)).
+    R (cQp.mut 1) |-- R (cQp.mut (1/2)) ** R (cQp.mut (1/2)).
   Proof. iIntros "[R1 R2]". by iFrame "R1 R2". Abort.
   Let split_const :
-    R (CV.const 1) |-- R (CV.const (1/2)) ** R (CV.const (1/2)).
+    R (cQp.const 1) |-- R (cQp.const (1/2)) ** R (cQp.const (1/2)).
   Proof. iIntros "[R1 R2]". by iFrame "R1 R2". Abort.
   Let split_mk c :
-    R (CV.mk c 1) |-- let Rhalf := R (CV.mk c (1/2)) in Rhalf ** Rhalf.
+    R (cQp.mk c 1) |-- let Rhalf := R (cQp.mk c (1/2)) in Rhalf ** Rhalf.
   Proof. iIntros "[R1 R2]". by iFrame "R1 R2". Abort.
   Let split_cv cv :
-    R cv |-- let Rhalf := R (CV.mk (CV.is_const cv) (CV.frac cv/2)) in Rhalf ** Rhalf.
+    R cv |-- let Rhalf := R (cQp.mk (cQp.is_const cv) (cQp.frac cv/2)) in Rhalf ** Rhalf.
   Proof. iIntros "[R1 R2]". by iFrame "R1 R2". Abort.
 
   (*
@@ -65,25 +65,25 @@ Section EXAMPLES.
   of) [q1 + q2].
   *)
 
-  Let split_½ : R (CV.mut (1/2)) |-- let Rhalf := R (CV.mut (1/4)) in Rhalf ** Rhalf.
+  Let split_½ : R (cQp.mut (1/2)) |-- let Rhalf := R (cQp.mut (1/4)) in Rhalf ** Rhalf.
   Proof. iIntros "[R1 R2]". by iFrame "R1 R2". Abort.
-  Let split_1 : R (CV.mut 1) |-- let Rhalf := R (CV.mut (1/2)) in Rhalf ** Rhalf.
+  Let split_1 : R (cQp.mut 1) |-- let Rhalf := R (cQp.mut (1/2)) in Rhalf ** Rhalf.
   Proof. iIntros "[R1 R2]". by iFrame "R1 R2". Abort.
-  Let split_q q : R (CV.mut q) |-- let Rhalf := R (CV.mut (q/2)) in Rhalf ** Rhalf.
+  Let split_q q : R (cQp.mut q) |-- let Rhalf := R (cQp.mut (q/2)) in Rhalf ** Rhalf.
   Proof. iIntros "[R1 R2]". by iFrame "R1 R2". Abort.
 
-  Let split_sum q1 q2 : R (CV.mut (q1 + q2)) |-- R (CV.mut q1) ** R (CV.mut q2).
+  Let split_sum q1 q2 : R (cQp.mut (q1 + q2)) |-- R (cQp.mut q1) ** R (cQp.mut q2).
   Proof. iIntros "[R1 R2]". by iFrame "R1 R2". Abort.
 
   Let split_mul_l p q1 q2 :
-    R (CV.mut (p * (q1 + q2))) |-- R (CV.mut (p * q1)) ** R (CV.mut (p * q2)).
+    R (cQp.mut (p * (q1 + q2))) |-- R (cQp.mut (p * q1)) ** R (cQp.mut (p * q2)).
   Proof. iIntros "[R1 R2]". by iFrame "R1 R2". Abort.
   Let split_mul_r p q1 q2 :
-    R (CV.mut ((q1 + q2) * p)) |-- R (CV.mut (q1 * p)) ** R (CV.mut (q2 * p)).
+    R (cQp.mut ((q1 + q2) * p)) |-- R (cQp.mut (q1 * p)) ** R (cQp.mut (q2 * p)).
   Proof. iIntros "[R1 R2]". by iFrame "R1 R2". Abort.
 
   Let split_div p q1 q2 :
-    R (CV.mut ((q1 + q2) / p)) |-- R (CV.mut (q1 / p)) ** R (CV.mut (q2 / p)).
+    R (cQp.mut ((q1 + q2) / p)) |-- R (cQp.mut (q1 / p)) ** R (cQp.mut (q2 / p)).
   Proof. iIntros "[R1 R2]". by iFrame "R1 R2". Abort.
 
   (**
@@ -98,115 +98,115 @@ Section EXAMPLES.
 
   (**
   Combining anything other than two variables expands [op] and
-  attempts to simplify the [CV.is_const] part and the [CV.is_frac]
+  attempts to simplify the [cQp.is_const] part and the [cQp.is_frac]
   part. (This example does not simplify.)
   *)
 
   Let combine_cv_mk cv c :
-    R cv ** R (CV.mk c (1/2)) |-- R (CV.mk (CV.is_const cv && c) (CV.frac cv + 1/2)).
+    R cv ** R (cQp.mk c (1/2)) |-- R (cQp.mk (cQp.is_const cv && c) (cQp.frac cv + 1/2)).
   Proof. iIntros "[R1 R2]"; iCombine "R1 R2" as "R". by iFrame "R". Abort.
   Let combine_mk_cv cv c :
-    R (CV.mk c (1/2)) ** R cv|-- R (CV.mk (c && CV.is_const cv) (1/2 + CV.frac cv)).
+    R (cQp.mk c (1/2)) ** R cv|-- R (cQp.mk (c && cQp.is_const cv) (1/2 + cQp.frac cv)).
   Proof. iIntros "[R1 R2]"; iCombine "R1 R2" as "R". by iFrame "R". Abort.
 
-  (** Simplifing [CV.is_const] given two concrete values *)
+  (** Simplifing [cQp.is_const] given two concrete values *)
 
   Let combine_mut_mut :
-    R (CV.mut (1/2)) ** R (CV.mut (1/2)) |-- R (CV.mut 1).
+    R (cQp.mut (1/2)) ** R (cQp.mut (1/2)) |-- R (cQp.mut 1).
   Proof. iIntros "[R1 R2]"; iCombine "R1 R2" as "R". by iFrame "R". Abort.
   Let combine_mut_const :
-    R (CV.mut (1/2)) ** R (CV.const (1/2)) |-- R (CV.mut 1).
+    R (cQp.mut (1/2)) ** R (cQp.const (1/2)) |-- R (cQp.mut 1).
   Proof. iIntros "[R1 R2]"; iCombine "R1 R2" as "R". by iFrame "R". Abort.
   Let combine_const_mut :
-    R (CV.const (1/2)) ** R (CV.mut (1/2)) |-- R (CV.mut 1).
+    R (cQp.const (1/2)) ** R (cQp.mut (1/2)) |-- R (cQp.mut 1).
   Proof. iIntros "[R1 R2]"; iCombine "R1 R2" as "R". by iFrame "R". Abort.
 
   Let combine_const_const :
-    R (CV.const (1/2)) ** R (CV.const (1/2)) |-- R (CV.const 1).
+    R (cQp.const (1/2)) ** R (cQp.const (1/2)) |-- R (cQp.const 1).
   Proof. iIntros "[R1 R2]"; iCombine "R1 R2" as "R". by iFrame "R". Abort.
 
-  (** Simplifing [CV.is_const] given one concrete value *)
+  (** Simplifing [cQp.is_const] given one concrete value *)
 
   Let combine_mut_var q cv :
-    R (CV.mut q) ** R cv |-- R (CV.mut (q + CV.frac cv)).
+    R (cQp.mut q) ** R cv |-- R (cQp.mut (q + cQp.frac cv)).
   Proof. iIntros "[R1 R2]"; iCombine "R1 R2" as "R". by iFrame "R". Abort.
   Let combine_var_mut q cv :
-    R cv ** R (CV.mut q) |-- R (CV.mut (CV.frac cv + q)).
+    R cv ** R (cQp.mut q) |-- R (cQp.mut (cQp.frac cv + q)).
   Proof. iIntros "[R1 R2]"; iCombine "R1 R2" as "R". by iFrame "R". Abort.
 
   Let combine_const_var q cv :
-    R (CV.const q) ** R cv |-- R (CV.mk (CV.is_const cv) (q + CV.frac cv)).
+    R (cQp.const q) ** R cv |-- R (cQp.mk (cQp.is_const cv) (q + cQp.frac cv)).
   Proof. iIntros "[R1 R2]"; iCombine "R1 R2" as "R". by iFrame "R". Abort.
   Let combine_var_const q cv :
-    R cv ** R (CV.const q) |-- R (CV.mk (CV.is_const cv) (CV.frac cv + q)).
+    R cv ** R (cQp.const q) |-- R (cQp.mk (cQp.is_const cv) (cQp.frac cv + q)).
   Proof. iIntros "[R1 R2]"; iCombine "R1 R2" as "R". by iFrame "R". Abort.
 
   Let combine_mut_mk c :
-    R (CV.mut (1/2)) ** R (CV.mk c (1/2)) |-- R (CV.mut 1).
+    R (cQp.mut (1/2)) ** R (cQp.mk c (1/2)) |-- R (cQp.mut 1).
   Proof. iIntros "[R1 R2]"; iCombine "R1 R2" as "R". by iFrame "R". Abort.
   Let combine_mk_mut c :
-    R (CV.mk c (1/2)) ** R (CV.mut (1/2)) |-- R (CV.mut 1).
+    R (cQp.mk c (1/2)) ** R (cQp.mut (1/2)) |-- R (cQp.mut 1).
   Proof. iIntros "[R1 R2]"; iCombine "R1 R2" as "R". by iFrame "R". Abort.
 
   Let combine_const_mk c :
-    R (CV.const (1/2)) ** R (CV.mk c (1/2)) |-- R (CV.mk c 1).
+    R (cQp.const (1/2)) ** R (cQp.mk c (1/2)) |-- R (cQp.mk c 1).
   Proof. iIntros "[R1 R2]"; iCombine "R1 R2" as "R". by iFrame "R". Abort.
   Let combine_mk_const c :
-    R (CV.mk c (1/2)) ** R (CV.const (1/2)) |-- R (CV.mk c 1).
+    R (cQp.mk c (1/2)) ** R (cQp.const (1/2)) |-- R (cQp.mk c 1).
   Proof. iIntros "[R1 R2]"; iCombine "R1 R2" as "R". by iFrame "R". Abort.
 
-  (** Simplifying [CV.is_const] given no concrete values *)
+  (** Simplifying [cQp.is_const] given no concrete values *)
 
   Let combine_cv cv :
-    let Rhalf := R (CV.mk (CV.is_const cv) (CV.frac cv/2)) in Rhalf ** Rhalf |-- R cv.
+    let Rhalf := R (cQp.mk (cQp.is_const cv) (cQp.frac cv/2)) in Rhalf ** Rhalf |-- R cv.
   Proof. iIntros "[R1 R2]"; iCombine "R1 R2" as "R". by iFrame "R". Abort.
 
   Let combine_mk c :
-    let Rhalf := R (CV.mk c (1/2)) in Rhalf ** Rhalf |-- R (CV.mk c 1).
+    let Rhalf := R (cQp.mk c (1/2)) in Rhalf ** Rhalf |-- R (cQp.mk c 1).
   Proof. iIntros "[R1 R2]"; iCombine "R1 R2" as "R". by iFrame "R". Abort.
 
   Let combine_cv_mk cv c q :
-    R cv ** R (CV.mk c q) |-- R (CV.mk (CV.is_const cv && c) (CV.frac cv + q)).
+    R cv ** R (cQp.mk c q) |-- R (cQp.mk (cQp.is_const cv && c) (cQp.frac cv + q)).
   Proof. iIntros "[R1 R2]"; iCombine "R1 R2" as "R". by iFrame "R". Abort.
   Let combine_mk_cv cv c q :
-    R (CV.mk c q) ** R cv |-- R (CV.mk (c && CV.is_const cv) (q + CV.frac cv)).
+    R (cQp.mk c q) ** R cv |-- R (cQp.mk (c && cQp.is_const cv) (q + cQp.frac cv)).
   Proof. iIntros "[R1 R2]"; iCombine "R1 R2" as "R". by iFrame "R". Abort.
 
   Let combine_mk_mk c1 c2 q1 q2 :
-    R (CV.mk c1 q1) ** R (CV.mk c2 q2) |-- R (CV.mk (c1 && c2) (q1 + q2)).
+    R (cQp.mk c1 q1) ** R (cQp.mk c2 q2) |-- R (cQp.mk (c1 && c2) (q1 + q2)).
   Proof. iIntros "[R1 R2]"; iCombine "R1 R2" as "R". by iFrame "R". Abort.
 
   (**
-  Simpifying [CV.frac] is pretty aggressive. We give a few examples.
+  Simpifying [cQp.frac] is pretty aggressive. We give a few examples.
   *)
 
-  Let combine_quarter q : R (CV.mut (q/4)) ** R (CV.mut (q/4)) |-- R (CV.mut (q/2)).
+  Let combine_quarter q : R (cQp.mut (q/4)) ** R (cQp.mut (q/4)) |-- R (cQp.mut (q/2)).
   Proof. iIntros "[R1 R2]"; iCombine "R1 R2" as "R". by iFrame "R". Abort.
-  Let combine_¼ : R (CV.mut (1/4)) ** R (CV.mut (1/4)) |-- R (CV.mut (1/2)).
-  Proof. iIntros "[R1 R2]"; iCombine "R1 R2" as "R". by iFrame "R". Abort.
-
-  Let combine_half q : R (CV.mut (q/2)) ** R (CV.mut (q/2)) |-- R (CV.mut q).
-  Proof. iIntros "[R1 R2]"; iCombine "R1 R2" as "R". by iFrame "R". Abort.
-  Let combine_½ : R (CV.mut (1/2)) ** R (CV.mut (1/2)) |-- R (CV.mut 1).
+  Let combine_¼ : R (cQp.mut (1/4)) ** R (cQp.mut (1/4)) |-- R (cQp.mut (1/2)).
   Proof. iIntros "[R1 R2]"; iCombine "R1 R2" as "R". by iFrame "R". Abort.
 
-  Let combine : R (CV.mut (1/4)) ** R (CV.mut (3/4)) |-- R (CV.mut 1).
+  Let combine_half q : R (cQp.mut (q/2)) ** R (cQp.mut (q/2)) |-- R (cQp.mut q).
   Proof. iIntros "[R1 R2]"; iCombine "R1 R2" as "R". by iFrame "R". Abort.
-  Let combine : R (CV.mut (3/4)) ** R (CV.mut (1/4)) |-- R (CV.mut 1).
+  Let combine_½ : R (cQp.mut (1/2)) ** R (cQp.mut (1/2)) |-- R (cQp.mut 1).
   Proof. iIntros "[R1 R2]"; iCombine "R1 R2" as "R". by iFrame "R". Abort.
 
-  Let combine : R (CV.mut (1/3)) ** R (CV.mut (2/3)) |-- R (CV.mut 1).
+  Let combine : R (cQp.mut (1/4)) ** R (cQp.mut (3/4)) |-- R (cQp.mut 1).
   Proof. iIntros "[R1 R2]"; iCombine "R1 R2" as "R". by iFrame "R". Abort.
-  Let combine : R (CV.mut (2/3)) ** R (CV.mut (1/3)) |-- R (CV.mut 1).
+  Let combine : R (cQp.mut (3/4)) ** R (cQp.mut (1/4)) |-- R (cQp.mut 1).
+  Proof. iIntros "[R1 R2]"; iCombine "R1 R2" as "R". by iFrame "R". Abort.
+
+  Let combine : R (cQp.mut (1/3)) ** R (cQp.mut (2/3)) |-- R (cQp.mut 1).
+  Proof. iIntros "[R1 R2]"; iCombine "R1 R2" as "R". by iFrame "R". Abort.
+  Let combine : R (cQp.mut (2/3)) ** R (cQp.mut (1/3)) |-- R (cQp.mut 1).
   Proof. iIntros "[R1 R2]"; iCombine "R1 R2" as "R". by iFrame "R". Abort.
 
   Let combine_mul_l p q1 q2 :
-    R (CV.mut (p * q1)) ** R (CV.mut (p * q2)) |-- R (CV.mut (p * (q1 + q2))).
+    R (cQp.mut (p * q1)) ** R (cQp.mut (p * q2)) |-- R (cQp.mut (p * (q1 + q2))).
   Proof. iIntros "[R1 R2]"; iCombine "R1 R2" as "R". by iFrame "R". Abort.
   Let combine_mul_r p q1 q2 :
-    R (CV.mut (q1 * p)) ** R (CV.mut (q2 * p)) |-- R (CV.mut ((q1 + q2) * p)).
+    R (cQp.mut (q1 * p)) ** R (cQp.mut (q2 * p)) |-- R (cQp.mut ((q1 + q2) * p)).
   Proof. iIntros "[R1 R2]"; iCombine "R1 R2" as "R". by iFrame "R". Abort.
   Let combine_div p q1 q2 :
-    R (CV.mut (q1 / p)) ** R (CV.mut (q2 / p)) |-- R (CV.mut ((q1 + q2) / p)).
+    R (cQp.mut (q1 / p)) ** R (cQp.mut (q2 / p)) |-- R (cQp.mut ((q1 + q2) / p)).
   Proof. iIntros "[R1 R2]"; iCombine "R1 R2" as "R". by iFrame "R". Abort.
 End EXAMPLES.
