theories/lang/cpp/bi/spec/cfrac_splittable.v
@@ -35,13 +35,13 @@ combined using XXX and addition on fractions; and
 
 Ltac solve_cfrac := solve [intros; split; apply _].
 
-Class CFracSplittable_0 {PROP : bi} (R : CV.t → PROP) : Prop := {
+Class CFracSplittable_0 {PROP : bi} (R : cQp.t → PROP) : Prop := {
   cfrac_splittable_0_fractional :> CFractional R;
   cfrac_splittable_0_timeless :> Timeless1 R;
   cfrac_splittable_0_frac_valid :> CFracValid0 R;
 }.
 Section cfrac_0.
-  Context {PROP : bi} (R : CV.t → PROP) `{!CFracSplittable_0 R}.
+  Context {PROP : bi} (R : cQp.t → PROP) `{!CFracSplittable_0 R}.
 
   #[global] Instance cfrac_splittable_0_as_fractional : AsCFractional0 R.
   Proof. solve_as_cfrac. Qed.
@@ -51,8 +51,8 @@ Section cfrac_0.
     (**
     TODO (Revisit if clients see similar problems): The shorter proof
     [iApply observe with "R"] does not work because the goal [[|
-    CV.frac q1 + CV.frac q2 ≤ 1 |]%Qp] does not match the observation
-    [[| CV.frac (q1 ⋅ q2) ≤ 1 |]%Qp] on the nose. Reconsider having
+    cQp.frac q1 + cQp.frac q2 ≤ 1 |]%Qp] does not match the observation
+    [[| cQp.frac (q1 ⋅ q2) ≤ 1 |]%Qp] on the nose. Reconsider having
     [iCombine] introduce [op].
     *)
     iDestruct (observe [| _ ≤ 1 |]%Qp with "R") as %?. auto.
@@ -60,7 +60,7 @@ Section cfrac_0.
 End cfrac_0.
 
 Section cfrac_1_gen.
-  Context {A} {PROP : bi} (R : CV.t → A → PROP).
+  Context {A} {PROP : bi} (R : cQp.t → A → PROP).
   Context {cfrac_splittable_1_frac_valid : CFracValid1 R}.
   Context {cfrac_splittable_1_as_fractional : AsCFractional1 R}.
 
@@ -73,7 +73,7 @@ Section cfrac_1_gen.
   Qed.
 
   #[global] Instance cfrac_splittable_1_agreef_excl_gen c q v1 v2 `{!AgreeCF1 R} :
-    Observe2 False (R (CV.mk c 1) v1) (R q v2).
+    Observe2 False (R (cQp.mk c 1) v1) (R q v2).
   Proof.
     iIntros "R1 R2".
     iDestruct (observe_2 [| _ ≤ 1 |]%Qp with "R1 R2") as %Hv.
@@ -81,16 +81,16 @@ Section cfrac_1_gen.
   Qed.
 
   #[global] Instance cfrac_splittable_1_agreef_excl c :
-    AgreeCF1 R → Exclusive1 (R (CV.mk c 1)) := _.
+    AgreeCF1 R → Exclusive1 (R (cQp.mk c 1)) := _.
 End cfrac_1_gen.
 
-Class CFracSplittable_1 {A} {PROP : bi} (R : CV.t → A → PROP) : Prop := {
+Class CFracSplittable_1 {A} {PROP : bi} (R : cQp.t → A → PROP) : Prop := {
   cfrac_splittable_1_fractional :> CFractional1 R;
   cfrac_splittable_1_timeless :> Timeless2 R;
   cfrac_splittable_1_frac_valid :> CFracValid1 R;
 }.
 Section cfrac_1.
-  Context {A} {PROP : bi} (R : CV.t → A → PROP) `{!CFracSplittable_1 R}.
+  Context {A} {PROP : bi} (R : cQp.t → A → PROP) `{!CFracSplittable_1 R}.
 
   #[global] Instance cfrac_splittable_1_as_fractional : AsCFractional1 R.
   Proof. solve_as_cfrac. Qed.
@@ -98,43 +98,43 @@ Section cfrac_1.
   Goal AgreeCF1 R -> CFrac2Valid1 R.
   Proof. apply _. Abort.
 
-  Goal ∀ c, AgreeCF1 R → Exclusive1 (R (CV.mk c 1)).
+  Goal ∀ c, AgreeCF1 R → Exclusive1 (R (cQp.mk c 1)).
   Proof. apply _. Abort.
 End cfrac_1.
 
-Class CFracSplittable_2 {A B} {PROP : bi} (R : CV.t → A → B → PROP) : Prop := {
+Class CFracSplittable_2 {A B} {PROP : bi} (R : cQp.t → A → B → PROP) : Prop := {
   cfrac_splittable_2_fractional :> CFractional2 R;
   cfrac_splittable_2_timeless :> Timeless3 R;
   cfrac_splittable_2_frac_valid :> CFracValid2 R;
 }.
 Section cfrac_2.
-  Context {A B} {PROP : bi} (R : CV.t → A → B → PROP) `{!CFracSplittable_2 R}.
+  Context {A B} {PROP : bi} (R : cQp.t → A → B → PROP) `{!CFracSplittable_2 R}.
 
   #[global] Instance cfrac_splittable_2_as_fractional : AsCFractional2 R.
   Proof. solve_as_cfrac. Qed.
 End cfrac_2.
 
 Class CFracSplittable_3 {A B C} {PROP : bi}
-    (R : CV.t → A → B → C → PROP) : Prop := {
+    (R : cQp.t → A → B → C → PROP) : Prop := {
   cfrac_splittable_3_fractional :> CFractional3 R;
   cfrac_splittable_3_timeless :> Timeless4 R;
   cfrac_splittable_3_frac_valid :> CFracValid3 R;
 }.
 Section cfrac_3.
-  Context {A B C} {PROP : bi} (R : CV.t → A → B → C → PROP) `{!CFracSplittable_3 R}.
+  Context {A B C} {PROP : bi} (R : cQp.t → A → B → C → PROP) `{!CFracSplittable_3 R}.
 
   #[global] Instance cfrac_splittable_3_as_fractional : AsCFractional3 R.
   Proof. solve_as_cfrac. Qed.
 End cfrac_3.
 
 Class CFracSplittable_4 {A B C D} {PROP : bi}
-    (R : CV.t → A → B → C → D → PROP) : Prop := {
+    (R : cQp.t → A → B → C → D → PROP) : Prop := {
   cfrac_splittable_4_fractional :> CFractional4 R;
   cfrac_splittable_4_timeless :> Timeless5 R;
   cfrac_splittable_4_frac_valid :> CFracValid4 R;
 }.
 Section cfrac_4.
-  Context {A B C D} {PROP : bi} (R : CV.t → A → B → C → D → PROP).
+  Context {A B C D} {PROP : bi} (R : cQp.t → A → B → C → D → PROP).
   Context `{!CFracSplittable_4 R}.
 
   #[global] Instance cfrac_splittable_4_as_fractional : AsCFractional4 R.
@@ -142,13 +142,13 @@ Section cfrac_4.
 End cfrac_4.
 
 Class CFracSplittable_5 {A B C D E} {PROP : bi}
-    (R : CV.t → A → B → C → D → E → PROP) : Prop := {
+    (R : cQp.t → A → B → C → D → E → PROP) : Prop := {
   cfrac_splittable_5_fractional :> CFractional5 R;
   cfrac_splittable_5_timeless :> Timeless6 R;
   cfrac_splittable_5_cfrac_valid :> CFracValid5 R;
 }.
 Section cfrac_5.
-  Context {A B C D E} {PROP : bi} (R : CV.t → A → B → C → D → E → PROP).
+  Context {A B C D E} {PROP : bi} (R : cQp.t → A → B → C → D → E → PROP).
   Context `{!CFracSplittable_5 R}.
 
   #[global] Instance cfrac_splittable_5_as_fractional : AsCFractional5 R.
