theories/lang/cpp/logic/layout.v
@@ -20,8 +20,8 @@ Section with_Σ.
   Context `{Σ : cpp_logic}.
 
   (** TODO move to pred.v *)
-  (* TODO swap the order of [CV.t] and [globname] *)
-  Axiom struct_paddingR : forall {σ:genv}, CV.t -> globname -> Rep.
+  (* TODO swap the order of [cQp.t] and [globname] *)
+  Axiom struct_paddingR : forall {σ:genv}, cQp.t -> globname -> Rep.
 
   (* [union_paddingR q cls active_member] is [q] fractional ownership of
      the union padding for union [cls] for the active member
@@ -29,9 +29,9 @@ Section with_Σ.
      is [None], otherwise it is [Some idx] where [idx] is the numeric
      index of member field.
 
-     TODO swap the order of [CV.t] and [globname].
+     TODO swap the order of [cQp.t] and [globname].
   *)
-  Axiom union_paddingR : forall {σ:genv}, CV.t -> globname -> option nat -> Rep.
+  Axiom union_paddingR : forall {σ:genv}, cQp.t -> globname -> option nat -> Rep.
 
   Context {σ : genv}.
 
@@ -77,7 +77,7 @@ Section with_Σ.
       Exists rs, rawsR q rs ** [| raw_bytes_of_struct σ cls rss rs |].
 
   #[local] Definition implicit_destruct_ty (ty : type) :=
-    anyR ty (CV.mut 1) |-- |={↑pred_ns}=> tblockR ty (CV.mut 1).
+    anyR ty (cQp.mut 1) |-- |={↑pred_ns}=> tblockR ty (cQp.mut 1).
 
   (** implicit destruction of a primitive *)
   Axiom implicit_destruct_int : forall sz sgn, Reduce (implicit_destruct_ty (Tnum sz sgn)).
@@ -95,10 +95,10 @@ Section with_Σ.
                 (R (erase_qualifiers fld.(mem_type)))) **
     (if has_vtable st (* this is almost certainly [false] if the
                          object is trivially destructible. *)
-     then identityR cls nil (CV.mut 1) (** NOTE this doesn't really work out because i generally
+     then identityR cls nil (cQp.mut 1) (** NOTE this doesn't really work out because i generally
                                    require a fancy update to forget the MDC. *)
      else emp)%I **
-    struct_paddingR (CV.mut 1) cls.
+    struct_paddingR (cQp.mut 1) cls.
 
 
   (** implicit destruction of an aggregate *)
@@ -107,23 +107,23 @@ Section with_Σ.
       glob_def σ cls = Some (Gstruct st) ->
       st.(s_trivially_destructible) ->
           type_ptrR (Tnamed cls)
-      |-- (Reduce (struct_def (fun ty => tblockR ty (CV.mut 1)) cls st)) -*
-          |={↑pred_ns}=> tblockR (Tnamed cls) (CV.mut 1).
+      |-- (Reduce (struct_def (fun ty => tblockR ty (cQp.mut 1)) cls st)) -*
+          |={↑pred_ns}=> tblockR (Tnamed cls) (cQp.mut 1).
 
   (** decompose a struct into its constituent fields and base classes.
    *)
   Axiom anyR_struct
   : forall cls st,
     glob_def σ cls = Some (Gstruct st) ->
-        anyR (Tnamed cls) (CV.mut 1)
-    -|- Reduce (struct_def (fun ty => anyR ty (CV.mut 1)) cls st).
+        anyR (Tnamed cls) (cQp.mut 1)
+    -|- Reduce (struct_def (fun ty => anyR ty (cQp.mut 1)) cls st).
 
   Definition union_def (R : type -> Rep) (cls : globname) (st : translation_unit.Union) : Rep :=
-    union_paddingR (CV.mut 1) cls None \\//
+    union_paddingR (cQp.mut 1) cls None \\//
     [∨list] idx↦it ∈ st.(u_fields),
        let f := _field {| f_name := it.(mem_name) ; f_type := cls |} in
        f |-> R (erase_qualifiers it.(mem_type)) **
-       union_paddingR (CV.mut 1) cls (Some idx).
+       union_paddingR (cQp.mut 1) cls (Some idx).
 
   (** implicit destruction of a union. *)
   Axiom implicit_destruct_union
@@ -131,7 +131,7 @@ Section with_Σ.
       glob_def σ cls = Some (Gunion un) ->
       un.(u_trivially_destructible) ->
           type_ptrR (Tnamed cls)
-      |-- (Reduce (union_def (fun ty => tblockR ty (CV.mut 1)) cls un)) -* |={↑pred_ns}=> tblockR (Tnamed cls) (CV.mut 1).
+      |-- (Reduce (union_def (fun ty => tblockR ty (cQp.mut 1)) cls un)) -* |={↑pred_ns}=> tblockR (Tnamed cls) (cQp.mut 1).
 
 (*
   (* the following rule would allow you to change the active entity in a union
@@ -152,11 +152,11 @@ Section with_Σ.
       glob_def resolve cls = Some (Gunion un) ->
 (*      un.(u_trivially_destructible) -> *)
       type_ptrR (Tnamed cls)
-      |-- (union_def (fun ty => tblockR ty (CV.mut 1)) cls un)
+      |-- (union_def (fun ty => tblockR ty (cQp.mut 1)) cls un)
       -* [∧ list] idx ↦ it ∈ un.(u_fields),
           let f := _field {| f_name := it.(mem_name) ; f_type := cls |} in
-          |={↑pred_ns}=> f |-> tblockR (erase_qualifiers it.(mem_type)) (CV.mut 1) **
-               union_paddingR resolve (CV.mut 1) cls (Some idx).
+          |={↑pred_ns}=> f |-> tblockR (erase_qualifiers it.(mem_type)) (cQp.mut 1) **
+               union_paddingR resolve (cQp.mut 1) cls (Some idx).
 *)
 
   (** decompose a union into the classical disjunction of the alternatives
@@ -164,8 +164,8 @@ Section with_Σ.
   Axiom anyR_union
   : forall (cls : globname) un,
     glob_def σ cls = Some (Gunion un) ->
-        anyR (Tnamed cls) (CV.mut 1)
-    -|- Reduce (union_def (fun ty => anyR ty (CV.mut 1)) cls un).
+        anyR (Tnamed cls) (cQp.mut 1)
+    -|- Reduce (union_def (fun ty => anyR ty (cQp.mut 1)) cls un).
 
  (** Proof requires the generalization of [anyR] to support aggregates (and arrays) *)
   Lemma anyR_array_0 t q :
