theories/lang/cpp/logic/rep.v
@@ -72,11 +72,11 @@ Section with_cpp.
     AsFractional (as_Rep (P q)) (λ q, as_Rep (P q)) q.
   Proof. constructor. done. apply _. Qed.
 
-  #[global] Instance as_Rep_cfractional {P : CV.t -> ptr -> mpred} :
+  #[global] Instance as_Rep_cfractional {P : cQp.t -> ptr -> mpred} :
     CFractional1 P ->
     CFractional (fun q => as_Rep (P q)).
   Proof. intros HP q1 q2. constructor =>p. by rewrite monPred_at_sep /= HP. Qed.
-  #[global] Instance as_Rep_as_cfractional (P : CV.t -> ptr -> mpred) q :
+  #[global] Instance as_Rep_as_cfractional (P : cQp.t -> ptr -> mpred) q :
     AsCFractional1 P ->
     AsCFractional (as_Rep (P q)) (λ q, as_Rep (P q)) q.
   Proof. solve_as_cfrac. Qed.
@@ -324,11 +324,11 @@ Section with_cpp.
     AsFractional (o |-> R) (λ q, o |-> r q) q.
   Proof. constructor. by rewrite -as_fractional. apply _. Qed.
 
-  #[global] Instance _offsetR_cfractional {R : CV.t -> Rep} o :
+  #[global] Instance _offsetR_cfractional {R : cQp.t -> Rep} o :
     CFractional R ->
     CFractional (fun q => _offsetR o (R q)).
   Proof. intros HR q1 q2. constructor =>p. by rewrite cfractional _offsetR_sep. Qed.
-  #[global] Instance _offsetR_as_cfractional o (P : Rep) (R : CV.t -> Rep) q :
+  #[global] Instance _offsetR_as_cfractional o (P : Rep) (R : cQp.t -> Rep) q :
     AsCFractional P R q ->
     AsCFractional (_offsetR o P) (λ q, _offsetR o (R q)) q.
   Proof. constructor. by rewrite -as_cfractional. apply _. Qed.
@@ -513,11 +513,11 @@ Section with_cpp.
     AsFractional (p |-> R) (λ q, p |-> r q) q.
   Proof. constructor. by rewrite -as_fractional. apply _. Qed.
 
-  #[global] Instance _at_cfractional {R : CV.t -> Rep} p :
+  #[global] Instance _at_cfractional {R : cQp.t -> Rep} p :
     CFractional R ->
     CFractional (fun q => _at p (R q)).
   Proof. intros HR q1 q2. by rewrite cfractional _at_sep. Qed.
-  #[global] Instance _at_as_cfractional p (P : Rep) (R : CV.t -> Rep) q :
+  #[global] Instance _at_as_cfractional p (P : Rep) (R : cQp.t -> Rep) q :
     AsCFractional P R q ->
     AsCFractional (_at p P) (λ q, _at p (R q)) q.
   Proof. constructor. by rewrite -as_cfractional. apply _. Qed.
@@ -584,10 +584,10 @@ Section with_cpp.
     AsFractional P Φ q →
     AsFractional (pureR P) (λ q, pureR (Φ q)) q.
   Proof. intros [??]. constructor. done. apply _. Qed.
-  #[global] Instance pureR_cfractional (P : CV.t → mpred) :
+  #[global] Instance pureR_cfractional (P : cQp.t → mpred) :
     CFractional P -> CFractional (fun q => pureR (P q)).
   Proof. apply _. Qed.
-  #[global] Instance pureR_as_cfractional (P : mpred) (F : CV.t -> mpred) q :
+  #[global] Instance pureR_as_cfractional (P : mpred) (F : cQp.t -> mpred) q :
     AsCFractional P F q →
     AsCFractional (pureR P) (fun q => pureR (F q)) q.
   Proof. intros [??]. constructor. done. apply _. Qed.
